tests/exceptions.v
@@ -6,7 +6,7 @@ Axiom block : M nat.
 Fail Definition block_fails := ltac:(mrun block).
 
 Definition block_raises_failure :=
-  ltac:(mrun (mtry block with [? s] Failure s => print s;; ret 0 end)).
+  ltac:(mrun (mtry block with StuckTerm => ret 0 end)).
 
 Example simple_ex :=
   ltac:(mrun (mtry raise exception with exception => ret 0 end)).
@@ -19,10 +19,10 @@ Example not_closed_but_closed (m : nat) :=
   ltac:(mrun (mtry raise (AnException m) with [? n] AnException n => ret n end)).
 
 Example nu_not_closed_raise_not_closed  :=
-  ltac:(mrun (mtry \nu x:nat, raise (AnException x) with [? s] ExceptionNotGround s => ret s end)).
+  ltac:(mrun (mtry \nu x:nat, raise (AnException x) with ExceptionNotGround => ret 0 end)).
 
 Example evar_not_closed_raise_not_closed  :=
-  ltac:(mrun (mtry e <- evar nat; raise (AnException e) with [? s] ExceptionNotGround s => ret s end)).
+  ltac:(mrun (mtry e <- evar nat; raise (AnException e) with ExceptionNotGround => ret 0 end)).
 
 Example evar_closed_is_fine  :=
   ltac:(mrun (mtry e <- evar nat; munify e 0 UniCoq;; raise (AnException e) with [? n] AnException n => ret n end)).
